Instantiated frame inference example with real resources

examples/lowstar_resources/FrameInference.fst
@@ -1,124 +1,127 @@
 module FrameInference
 open FStar.Tactics
 module T = FStar.Tactics
-assume
-val resource : Type u#1
+module U32 = FStar.UInt32
 
-assume
-val emp : resource
+module R = LowStar.Resource
+module A = LowStar.Array
+module AR = LowStar.RST.Array
+module RST = LowStar.RST
+module Tac = LowStar.RST.Tactics
 
-assume
-val ptr (a:Type0) : Type0
+let cmd (r1:R.resource) (r2:R.resource) = unit -> RST.RST unit r1 (fun _ -> r2) (fun _ -> True) (fun _ _ _ -> True)
 
-assume
-val ptr_resource (x:ptr 'a) : resource
-
-assume
-val ( ** ) (r1 r2:resource) : resource
-
-assume
-val emp_unit (r1 :resource)
-  : Lemma (r1 ** emp == r1)
-
-assume
-val commutative (r1 r2:resource)
-  : Lemma (r1 ** r2 == r2 ** r1)
-
-assume
-val associative (r1 r2 r3:resource)
-  : Lemma (r1 ** (r2 ** r3) == (r1 ** r2) ** r3)
-
-[@unifier_hint_injective]
-assume
-val cmd (r1:resource) (r2:resource) : Type
-
-assume
-val ( >> ) (#p #q #r : resource) (f:cmd p q) (g:cmd q r)
+let compose (#p #q #r : R.resource)
+  (f: cmd p q)
+  (g: cmd q r)
   : cmd p r
+  = fun _ -> g (f ())
 
-assume
-val frame (#frame #p #q : resource) (f:cmd p q)
-  : cmd (frame ** p) (frame ** q)
+let ( >> ) (#p #q #r : R.resource)
+  (f: cmd p q)
+  (g: cmd q r)
+  : cmd p r
+  = compose f g
 
-assume
-val frame_delta (pre p post q : resource) : Type
+let frame (#frame #p #q : R.resource) (f:cmd p q) : cmd R.(frame <*> p) R.(frame <*> q)
+  = fun _ ->
+   RST.rst_frame
+     R.(frame <*> p)
+     #p
+     #unit
+     (fun _ -> R.(frame <*> q))
+     #(fun _ -> q)
+     #frame
+     #(fun _ -> True)
+     #(fun _ _ _ -> True)
+     (fun _ -> f ())
 
-assume
-val frame2
-    (#pre #post #p #q : resource)
-    (#delta:frame_delta pre p post q)
+
+let frame2
+    (#pre #post #p #q : R.resource)
+    (#delta: R.resource{Tac.frame_delta pre p (fun _ -> post) (fun _ -> q) delta})
     (f:cmd p q)
   : cmd pre post
+= fun _ ->
+   RST.rst_frame
+     pre
+     #p
+     #unit
+     (fun _ -> post)
+     #(fun _ -> q)
+     #(magic ())//delta
+     #(fun _ -> True)
+     #(fun _ _ _ -> True)
+     (fun _ -> f ())
+
+let f (b: A.array U32.t) : cmd (AR.array_resource b) (AR.array_resource b) =
+  (fun _ -> ignore (AR.index b 0ul))
+
+let test0 (b1: A.array U32.t) (b2: A.array U32.t)
+  : cmd R.(AR.array_resource b1 <*> AR.array_resource b2) R.(AR.array_resource b1 <*> AR.array_resource b2)
+ =
+  compose (frame (f b2)) (frame  (f b2))
 
 
-assume
-val frame_delta_refl (pre p q : resource) : frame_delta pre p pre q
-
-////////////////////////////////////////////////////////////////////////////////
-
-assume val r1 : resource
-assume val r2 : resource
-assume val r3 : resource
-assume val r4 : resource
-assume val r5 : resource
-
-assume val f1: cmd r1 r1
-assume val f2: cmd r2 r2
-assume val f3: cmd r3 r3
-assume val f4: cmd r4 r4
-assume val f5: cmd r5 r5
 
 
-let test0 : cmd (r1 ** r2) (r1 ** r2) =
-  frame f2 >>
-  frame f2
-
-// let test1 : cmd (r1 ** r2) (r1 ** r2) =
-//   frame f1 >>
-//   frame f2
+[@expect_failure]
+let test1 (b1: A.array U32.t) (b2: A.array U32.t)
+  : cmd R.(AR.array_resource b1 <*> AR.array_resource b2) R.(AR.array_resource b1 <*> AR.array_resource b2)
+ =
+  compose #R.(AR.array_resource b1 <*> AR.array_resource b2) # R.(AR.array_resource b1 <*> AR.array_resource b2)
+  (frame #(AR.array_resource b2) #(AR.array_resource b1) #(AR.array_resource b1) (f b1))
+  (frame #(AR.array_resource b1) #(AR.array_resource b2) #(AR.array_resource b2) (f b2))
 
 [@resolve_implicits]
 let resolve_tac () : Tac unit =
   T.dump "Start!";
   let _ = T.repeat (fun () ->
-    T.apply (`frame_delta_refl);
+    T.apply (`Tac.resolve_frame_delta);
     T.dump "Next")
   in
   ()
 
 
-let test1 (b:bool)
-  : cmd (r1 ** r2 ** r3 ** r4 ** r5)
-        (r1 ** r2 ** r3 ** r4 ** r5)
+[@expect_failure]
+let test2 (b1: A.array U32.t) (b2: A.array U32.t) (b3: A.array U32.t) (b4: A.array U32.t) (b5: A.array U32.t)
+  : cmd R.(AR.array_resource b1 <*> AR.array_resource b2 <*> AR.array_resource b3 <*> AR.array_resource b4 <*> AR.array_resource b5)
+        R.(AR.array_resource b1 <*> AR.array_resource b2 <*> AR.array_resource b3 <*> AR.array_resource b4 <*> AR.array_resource b5)
   =
-  frame2 f1 >>
-  frame2 f2 >>
-  frame2 f3 >>
-  frame2 f4 >>
-  frame2 f5
-
-  // >>
-  // (if b then
-  //   frame2 f3 >>
-  //   frame2 f4
-  //  else frame2 f5)
-
+  frame2 (f b1) >>
+  frame2 (f b2) >>
+  frame2 (f b3) >>
+  frame2 (f b4) >>
+  frame2 (f b5)
 
 #set-options "--print_implicits"
 
 
-assume
-val frame3
-    (#pre #post #p #q : resource)
-    (#[T.apply (`frame_delta_refl)] delta:frame_delta pre p post q)
+let frame3
+    (#pre #post #p #q : R.resource)
+    (#[T.apply (`Tac.resolve_delta)] delta:R.resource{Tac.frame_delta pre p (fun _ -> post) (fun _ -> q) delta})
     (f:cmd p q)
   : cmd pre post
-
-let test2
-  : cmd (r1 ** r2) (r1 ** r2)
   =
-  frame3 f1 >>
-  frame3 f2 >>
-  frame3 f3 >>
-  frame3 f4 >>
-  frame3 f5
+   fun _ ->
+   RST.rst_frame
+     pre
+     #p
+     #unit
+     (fun _ -> post)
+     #(fun _ -> q)
+     #(magic ())//delta
+     #(fun _ -> True)
+     #(fun _ _ _ -> True)
+     (fun _ -> f ())
+
+[@expect_failure]
+let test3 (b1: A.array U32.t) (b2: A.array U32.t) (b3: A.array U32.t) (b4: A.array U32.t) (b5: A.array U32.t)
+  : cmd R.(AR.array_resource b1 <*> AR.array_resource b2 <*> AR.array_resource b3 <*> AR.array_resource b4 <*> AR.array_resource b5)
+        R.(AR.array_resource b1 <*> AR.array_resource b2 <*> AR.array_resource b3 <*> AR.array_resource b4 <*> AR.array_resource b5)
+  =
+  frame3 (f b1) >>
+  frame3 (f b2) >>
+  frame3 (f b3) >>
+  frame3 (f b4) >>
+  frame3 (f b5)
